CppFormalization/Cpp2/Static/NoDeclareObj.lean
@@ -1,0 +1,48 @@
+import CppFormalization.Cpp2.Semantics.Stmt
+
+namespace Cpp
+
+mutual
+
+inductive NoDeclareObjStmt : CppStmt → Prop where
+  | skip :
+      NoDeclareObjStmt .skip
+  | exprStmt {e : ValExpr} :
+      NoDeclareObjStmt (.exprStmt e)
+  | assign {p : PlaceExpr} {e : ValExpr} :
+      NoDeclareObjStmt (.assign p e)
+  | declareRef {τ : CppType} {x : Ident} {p : PlaceExpr} :
+      NoDeclareObjStmt (.declareRef τ x p)
+  | seq {s t : CppStmt} :
+      NoDeclareObjStmt s →
+      NoDeclareObjStmt t →
+      NoDeclareObjStmt (.seq s t)
+  | ite {c : ValExpr} {s t : CppStmt} :
+      NoDeclareObjStmt s →
+      NoDeclareObjStmt t →
+      NoDeclareObjStmt (.ite c s t)
+  | whileStmt {c : ValExpr} {body : CppStmt} :
+      NoDeclareObjStmt body →
+      NoDeclareObjStmt (.whileStmt c body)
+  | block {ss : StmtBlock} :
+      NoDeclareObjBlock ss →
+      NoDeclareObjStmt (.block ss)
+  | breakStmt :
+      NoDeclareObjStmt .breakStmt
+  | continueStmt :
+      NoDeclareObjStmt .continueStmt
+  | returnStmt {oe : Option ValExpr} :
+      NoDeclareObjStmt (.returnStmt oe)
+
+inductive NoDeclareObjBlock : StmtBlock → Prop where
+  | nil :
+      NoDeclareObjBlock .nil
+  | cons {s : CppStmt} {ss : StmtBlock} :
+      NoDeclareObjStmt s →
+      NoDeclareObjBlock ss →
+      NoDeclareObjBlock (.cons s ss)
+
+end
+
+
+end Cpp
